InferMatch.v
@@ -3,6 +3,7 @@ Require Import Coq.Strings.String.
 Require Export SystemFR.StepTactics.
 Require Export SystemFR.ErasedRecGen.
 Require Export SystemFR.ErasedSingleton.
+Require Export SystemFR.SubtypeList.
 
 Opaque reducible_values.
 
@@ -18,7 +19,11 @@ Lemma evaluate_list_match:
     [ ρ | v : List ]v -> (
       (v = tnil /\ star scbv_step (list_match v t2 t3) t2) \/
       (exists h l,
+         closed_value h /\
+         closed_value l /\
          v = tcons h l /\
+         [ ρ | h : T_top ] /\
+         [ ρ | l : List ] /\
          [ list_match v t2 t3 ≡ open 0 (open 1 t3 h) l ]
       )
     ).
@@ -26,10 +31,12 @@ Proof.
   unfold List, list_match.
   intros.
   apply (reducible_values_unfold_gen _ _ _ _ 0) in H6;
-    repeat step || simp_spos || simp_red_top_level_hyp.
+    repeat step || simp_spos.
+    simp_red_top_level_hyp; repeat step.
 
-  - left; steps; one_step.
-  - right; eexists; eexists; steps.
+  - simp_red_top_level_hyp; left; steps; one_step.
+  - simp_red_top_level_hyp; right; steps.
+    eexists; eexists; repeat step || simp_red_goal; t_closer; eauto using reducible_value_expr.
     apply equivalent_trans with (open 0 (open 1 t3 (pi1 (pp a b))) (pi2 (pp a b))).
     + equivalent_star;
         eauto 3 with erased step_tactic;
@@ -38,49 +45,203 @@ Proof.
 
       apply star_one.
       eapply scbv_step_same.
-      apply SPBetaMatchRight; t_closer.
-      rewrite open_shift_open2; steps; t_closer;
-        eauto 3 with wf step_tactic.
-      rewrite no_shift_open; t_closer.
-      rewrite open_shift_open2; steps; t_closer;
-        eauto 3 with wf step_tactic.
+      * apply SPBetaMatchRight; t_closer.
+      * rewrite open_shift_open3; steps; t_closer;
+          eauto 3 with wf step_tactic.
+        rewrite open_shift_open4; steps; t_closer;
+          eauto 3 with wf step_tactic.
+        rewrite no_shift_open; t_closer.
+        rewrite no_shift_open; t_closer.
+        rewrite open_twice; steps; t_closer.
 
-      2
-    eauto with smallstep.
-    apply Trans.
-    one_step.
+    + eapply equivalent_trans.
+      * apply equivalent_context; steps;
+          try solve [ apply is_erased_open; steps; t_closer ];
+          try solve [ apply wf_open; steps; t_closer ];
+          try solve [ apply fv_nils_open; steps; t_closer ].
+        apply equivalent_star; repeat step || list_utils; t_closer.
+        apply star_one.
+        constructor; t_closer.
+      * rewrite (swap_term_holes_open t3); steps; t_closer.
+        rewrite (swap_term_holes_open t3); steps; t_closer.
+        apply equivalent_context; steps;
+          try solve [ apply is_erased_open; steps; t_closer ];
+          try solve [ apply wf_open; steps; t_closer ];
+          try solve [ apply fv_nils_open; steps; t_closer ];
+          try solve [ apply wf_open; steps; t_closer; eauto with wf ].
+        apply equivalent_star; repeat step || list_utils; t_closer.
+        apply star_one.
+        constructor; t_closer.
+Qed.
 
+Ltac evaluate_list_match :=
+  match goal with
+  | H: valid_interpretation ?ρ |- context[list_match ?v ?t2 ?t3] =>
+    poseNew (Mark (v, t2, t3) "evaluate_list_match");
+    unshelve epose proof (evaluate_list_match ρ v t2 t3 _ _ _ _ _ _ _ _)
+  end.
 
-    open_none; auto.
+Lemma evaluate_list_match_scrut:
+  forall t t' t2 t3,
+    star scbv_step t t' ->
+    star scbv_step (list_match t t2 t3) (list_match t' t2 t3).
+Proof.
+  unfold list_match; steps; eauto with cbvlemmas.
+Qed.
 
 Opaque list_match.
-Opaque List_Match.
 
-  
-  
-  simp_red; steps.
-  
+Lemma reducible_union_left:
+  forall ρ t T1 T2,
+    valid_interpretation ρ ->
+    [ ρ | t : T1 ] ->
+    [ ρ | t : T_union T1 T2 ].
+Proof.
+  unfold reducible, reduces_to; steps.
+  eexists; repeat step || simp_red; eauto using reducible_values_closed.
+Qed.
 
-  
-  intros.
-  unfold List
-  repeat step || simp_red.
+Lemma reducible_union_right:
+  forall ρ t T1 T2,
+    valid_interpretation ρ ->
+    [ ρ | t : T2 ] ->
+    [ ρ | t : T_union T1 T2 ].
+Proof.
+  unfold reducible, reduces_to; steps.
+  eexists; repeat step || simp_red; eauto using reducible_values_closed.
+Qed.
 
+Lemma reducible_exists:
+  forall ρ t t' T1 T2,
+    valid_interpretation ρ ->
+    is_erased_type T2 ->
+    wf T2 1 ->
+    pfv T2 term_var = nil ->
+    [ ρ | t' : T1 ] ->
+    [ ρ | t : open 0 T2 t' ] ->
+    [ ρ | t : T_exists T1 T2 ].
+Proof.
+  unfold reducible, reduces_to;
+    repeat step.
+  exists v; repeat step || simp_red; eauto using reducible_values_closed.
+  exists v0; repeat step; t_closer.
+  eapply reducibility_values_ltr; eauto; steps; t_closer.
+Qed.
 
-Lemma tmatch:
-  forall ρ t t2 t3 T2 T3,
-    [ ρ | t : List ] ->
+Lemma tmatch_value:
+  forall ρ v t2 t3 T2 T3,
+    valid_interpretation ρ ->
+    wf t3 2 ->
+    wf T2 0 ->
+    wf T3 2 ->
+    is_erased_term t2 ->
+    is_erased_term t3 ->
+    is_erased_type T2 ->
+    is_erased_type T3 ->
+    pfv t2 term_var = nil ->
+    pfv t3 term_var = nil ->
+    pfv T2 term_var = nil ->
+    pfv T3 term_var = nil ->
+    [ ρ | v : List ]v ->
     [ ρ | t2 : T2 ] ->
     (forall h t, [ ρ | h : T_top ] -> [ ρ | t : List ] ->
             [ ρ | open 0 (open 1 t3 h) t : open 0 (open 1 T3 h) t ]) ->
+    [ ρ | list_match v t2 t3 : List_Match v T2 T3 ].
+Proof.
+  intros; evaluate_list_match; steps;
+    eauto with wf.
+
+  - eapply star_backstep_reducible; eauto;
+      repeat step || apply wf_list_match || apply is_erased_term_list_match ||
+             apply pfv_list_match;
+      eauto with wf.
+    unfold List_Match.
+    apply reducible_union_left; auto.
+    apply reducible_type_refine with uu; repeat step || simp_red || apply reducible_value_expr;
+      eauto using equivalent_refl with step_tactic.
+
+  - eapply reducibility_equivalent2; eauto using equivalent_sym;
+      repeat step || list_utils; t_closer.
+    unfold List_Match.
+    apply reducible_union_right; auto.
+    apply reducible_exists with h; repeat step || open_none; t_closer.
+    apply reducible_exists with l; repeat step || open_none; t_closer.
+    apply reducible_type_refine with uu; repeat step || open_none; t_closer.
+    apply reducible_value_expr; repeat step || simp_red_goal.
+    apply equivalent_refl; steps; t_closer.
+Qed.
+
+Lemma tmatch:
+  forall ρ t t2 t3 T2 T3,
+    valid_interpretation ρ ->
+    wf t3 2 ->
+    wf T2 0 ->
+    wf T3 2 ->
+    is_erased_term t2 ->
+    is_erased_term t3 ->
+    is_erased_type T2 ->
+    is_erased_type T3 ->
+    pfv t2 term_var = nil ->
+    pfv t3 term_var = nil ->
+    pfv T2 term_var = nil ->
+    pfv T3 term_var = nil ->
+    [ ρ | t : List ] ->
+    [ ρ | t2 : T2 ] ->
+    (forall h t, [ ρ | h : T_top ]v -> [ ρ | t : List ]v ->
+            [ ρ | open 0 (open 1 t3 h) t : open 0 (open 1 T3 h) t ]) ->
     [ ρ | list_match t t2 t3 : List_Match t T2 T3 ].
 Proof.
-Admitted.
+  intros.
+  unfold reducible, reduces_to in H11; steps.
+  apply reducibility_equivalent2 with (list_match v t2 t3); steps; t_closer.
+  - apply equivalent_sym.
+    equivalent_star;
+      repeat step || apply is_erased_term_list_match || apply wf_list_match || apply pfv_list_match;
+      eauto using evaluate_list_match_scrut;
+      t_closer.
+  - apply subtype_reducible with (List_Match v T2 T3).
+    + apply tmatch_value; steps.
+      unfold reducible, reduces_to in H11; steps.
+      unfold reducible, reduces_to in H17; steps.
+      eapply reducibility_equivalent2 with (open 0 (open 1 t3 h) v1);
+        repeat step || apply is_erased_type_open || apply equivalent_context ||
+               apply wf_open || apply fv_nils_open;
+        t_closer;
+        try solve [ apply equivalent_sym; equivalent_star ].
+      eapply reducibility_rtl; steps; eauto; t_closer.
+      rewrite swap_term_holes_open; steps; t_closer.
+      eapply reducibility_equivalent2 with (open 0 (open 1 (swap_term_holes t3 0 1) v1) v0);
+        repeat step ||
+               apply is_erased_type_open || apply is_erased_open ||
+               apply equivalent_context || apply wf_swap_term_holes_3 ||
+               apply wf_open || apply fv_nils_open;
+        t_closer;
+        try solve [ apply equivalent_sym; equivalent_star ].
+      rewrite (swap_term_holes_open T3); steps; t_closer.
+      eapply reducibility_rtl; eauto;
+      repeat step || apply is_erased_type_open || apply fv_nils_open; eauto; t_closer.
+      rewrite <- (swap_term_holes_open t3); steps; t_closer.
+      rewrite <- (swap_term_holes_open T3); steps; t_closer.
+    + apply subtype_list_match_scrut; steps.
+      apply equivalent_sym; equivalent_star.
+Qed.
 
 Lemma open_tmatch_helper:
   forall Θ Γ t t2 t3 T2 T3 x1 x2,
-    ~ x1 ∈ support Γ ->
-    ~ x2 ∈ support Γ ->
+    ~ x1 ∈ pfv_context Γ term_var ->
+    ~ x2 ∈ pfv_context Γ term_var ->
+    x1 <> x2 ->
+    wf t3 2 ->
+    wf T2 0 ->
+    wf T3 2 ->
+    is_erased_term t2 ->
+    is_erased_term t3 ->
+    is_erased_type T2 ->
+    is_erased_type T3 ->
+    subset (fv t2) (support Γ) ->
+    subset (fv t3) (support Γ) ->
+    subset (fv T2) (support Γ) ->
+    subset (fv T3) (support Γ) ->
     [ Θ; Γ ⊨ t : List ] ->
     [ Θ; Γ ⊨ t2 : T2 ] ->
     [ Θ; (x1, T_top) :: (x2, List) :: Γ ⊨
@@ -91,13 +252,29 @@ Proof.
   unfold open_reducible;
     repeat step || apply tmatch ||
            rewrite substitute_list_match || rewrite substitute_List_Match;
-    eauto with wf.
-Admitted.
+    t_closer.
+
+  unshelve epose proof (H15 ρ ((x1, h) :: (x2, t0) :: lterms) _ _ _);
+    repeat step || apply SatCons || t_substitutions;
+    t_closer.
+Qed.
 
 Lemma open_tmatch:
   forall Γ t t2 t3 T2 T3 x1 x2,
-    ~ x1 ∈ support Γ ->
-    ~ x2 ∈ support Γ ->
+    ~ x1 ∈ pfv_context Γ term_var ->
+    ~ x2 ∈ pfv_context Γ term_var ->
+    x1 <> x2 ->
+    wf t3 2 ->
+    wf T2 0 ->
+    wf T3 2 ->
+    is_erased_term t2 ->
+    is_erased_term t3 ->
+    is_erased_type T2 ->
+    is_erased_type T3 ->
+    subset (fv t2) (support Γ) ->
+    subset (fv t3) (support Γ) ->
+    subset (fv T2) (support Γ) ->
+    subset (fv T3) (support Γ) ->
     [ Γ ⊨ t : List ] ->
     [ Γ ⊨ t2 : T2 ] ->
     [ (x1, T_top) :: (x2, List) :: Γ ⊨
