SubtypeList.v
@@ -57,3 +57,48 @@ Lemma open_subcons:
 Proof.
   eauto using open_subcons_helper.
 Qed.
+
+Lemma subtype_list_match_scrut:
+  forall ρ t t' T2 T3,
+    valid_interpretation ρ ->
+    is_erased_type T2 ->
+    is_erased_type T3 ->
+    wf T2 0 ->
+    wf T3 2 ->
+    pfv T2 term_var = nil ->
+    pfv T3 term_var = nil ->
+    [ t ≡ t' ] ->
+    [ ρ | List_Match t T2 T3 <: List_Match t' T2 T3 ].
+Proof.
+  unfold List_Match, subtype; intros.
+  unshelve epose proof (reducibility_open_equivalent
+   (T_union
+      (T_type_refine T2 (T_equiv (lvar 1 term_var) tnil))
+      (T_exists T_top
+        (T_exists List
+          (T_type_refine T3
+            (T_equiv (lvar 3 term_var) (tcons (lvar 2 term_var) (lvar 1 term_var)))))))
+   t t' ρ v _ _ _ _ _ _);
+    repeat step || list_utils || open_none;
+    t_closer.
+Qed.
+
+Opaque List_Match.
+
+Lemma open_sub_list_match_scrut:
+  forall Γ t t' T2 T3,
+    is_erased_type T2 ->
+    is_erased_type T3 ->
+    wf T2 0 ->
+    wf T3 2 ->
+    pfv T2 term_var = nil ->
+    pfv T3 term_var = nil ->
+    [ Γ ⊨ t ≡ t' ] ->
+    [ Γ ⊨ List_Match t T2 T3 = List_Match t' T2 T3 ].
+Proof.
+  unfold open_equivalent_types, equivalent_types, open_equivalent;
+    repeat step || rewrite substitute_List_Match in * by eauto with wf.
+  - eapply subtype_list_match_scrut; steps; eauto with erased wf fv.
+  - eapply subtype_list_match_scrut; steps; eauto with erased wf fv;
+      eauto using equivalent_sym.
+Qed.
